src/Util/Streams.dfy
@@ -72,11 +72,11 @@ module Streams {
     }
 
     // Read exactly `n` bytes, if possible; otherwise, fail.
-    method ReadExact(n: nat) returns (ret: Result<seq<uint8>>)
+    method ReadExact(n: nat) returns (res: Result<seq<uint8>>)
       requires Valid()
       modifies this
       ensures Valid()
-      ensures match ret
+      ensures match res
         case Success(bytes) => |bytes| == n
         case Failure(_) => true
     {
@@ -88,14 +88,36 @@ module Streams {
       }
     }
 
+    // Read exactly 1 byte, if possible, and return as a uint8; otherwise, fail.
+    method ReadByte() returns (res: Result<uint8>)
+      requires Valid()
+      modifies this
+      ensures Valid()
+    {
+      var bytes :- ReadExact(1);
+      var n := bytes[0];
+      return Success(n);
+    }
+
     // Read exactly 2 bytes, if possible, and return as a uint16; otherwise, fail.
-    method ReadUInt16() returns (ret: Result<uint16>)
+    method ReadUInt16() returns (res: Result<uint16>)
       requires Valid()
       modifies this
       ensures Valid()
     {
       var bytes :- ReadExact(2);
       var n := SeqToUInt16(bytes);
+      return Success(n);
+    }
+
+    // Read exactly 4 bytes, if possible, and return as a uint32; otherwise, fail.
+    method ReadUInt32() returns (res: Result<uint32>)
+      requires Valid()
+      modifies this
+      ensures Valid()
+    {
+      var bytes :- ReadExact(4);
+      var n := SeqToUInt32(bytes);
       return Success(n);
     }
   }
@@ -111,119 +133,113 @@ module Streams {
       this in Repr
     }
 
-    function method Capacity(): nat  // An upper bound on the amount of data the stream can accept on Write
+    predicate method HasRemainingCapacity(n: nat)  // Compare with an upper bound on the amount of data the stream can accept on Write
       requires Valid()
       reads this
     {
-      0 // TODO?
+      true
     }
 
     constructor()
-      ensures Valid()
+      ensures Valid() && fresh(Repr)
     {
       data := [];
       Repr := {this};
     }
 
-    method Write(a: array<uint8>, off: nat, req: nat) returns (res: Result<nat>)
+    method Write(a: array<uint8>, off: nat, len: nat) returns (res: Result<nat>)
       requires Valid() && a !in Repr
-      requires off + req <= a.Length
+      requires off + len <= a.Length
       modifies `data
       ensures Valid()
       ensures match res
-        case Success(len_written) =>
-          if old(Capacity()) == 0 then
-            len_written == 0
-          else
-            && len_written == min(req, old(Capacity()))
-            && data == old(data) + a[off..off+req]
-        case Failure(e) => true
-    {
-      if off == a.Length || Capacity() == 0 {
-        return Success(0);
-      } else {
-        var n := min(req, Capacity());
-        data := data + a[off..off+req];
-        return Success(n);
-      }
-    }
-
-    method WriteSimple(a: array<uint8>) returns (res: Result<nat>)
-      requires Valid() && a !in Repr
-      modifies `data
-      ensures Valid()
-      ensures match res
-        case Success(len_written) =>
-            && len_written == a.Length
-            && data[..] == old(data) + a[..]
+        case Success(lengthWritten) =>
+          && old(HasRemainingCapacity(len))
+          && lengthWritten == len
+          && data == old(data) + a[off..][..len]
         case Failure(e) => unchanged(`data)
     {
-      if a.Length <= Capacity() {
-        data := data + a[..];
-        return Success(a.Length);
+      if HasRemainingCapacity(len) {
+        data := data + a[off..off + len];
+        return Success(len);
       } else {
-        return Failure("IO Error: Reached end of stream.");
+        return Failure("IO Error: Stream capacity exceeded.");
       }
     }
 
-    method WriteSimpleSeq(a: seq<uint8>) returns (res: Result<nat>)
+    method WriteSeq(bytes: seq<uint8>) returns (res: Result<nat>)
       requires Valid()
       modifies `data
       ensures Valid()
       ensures match res
-        case Success(len_written) =>
-            && len_written == |a|
-            && data[..] == old(data) + a
+        case Success(lengthWritten) =>
+          && old(HasRemainingCapacity(|bytes|))
+          && lengthWritten == |bytes|
+          && data == old(data) + bytes
         case Failure(e) => unchanged(`data)
     {
-      if |a| <= Capacity() {
-        data := data + a;
-        return Success(|a|);
+      if HasRemainingCapacity(|bytes|) {
+        data := data + bytes;
+        return Success(|bytes|);
       } else {
-        return Failure("IO Error: Reached end of stream.");
+        return Failure("IO Error: Stream capacity exceeded.");
       }
     }
 
-    method WriteSingleByte(a: uint8) returns (res: Result<nat>)
+    method WriteByte(n: uint8) returns (res: Result<nat>)
       requires Valid()
       modifies `data
       ensures Valid()
       ensures match res
-        case Success(len_written) =>
-          if old(Capacity()) == 0 then
-            len_written == 0
-          else
-            && len_written == 1
-            && data == old(data) + [a]
-            // Dafny->Boogie drops an old: https://github.com/dafny-lang/dafny/issues/320
-            //&& data[..] == old(data)[.. old(pos)] + [a] + old(data)[old(pos) + 1 ..]
+        case Success(lengthWritten) =>
+          && old(HasRemainingCapacity(1))
+          && lengthWritten == 1
+          && data == old(data) + [n]
         case Failure(e) => unchanged(`data)
     {
-      if Capacity() == 0 {
-        return Success(0);
-      } else {
-        data := data + [a];
-        return Success(1);
-      }
-    }
-
-    method WriteSingleByteSimple(a: uint8) returns (res: Result<nat>)
-      requires Valid()
-      modifies `data
-      ensures Valid()
-      ensures match res
-        case Success(len_written) =>
-            len_written == 1
-            && data == old(data) + [a]
-            // Dafny->Boogie drops an old: https://github.com/dafny-lang/dafny/issues/320
-            //&& data[..] == old(data)[.. old(pos)] + [a] + old(data)[old(pos) + 1 ..]
-        case Failure(e) => unchanged(`data)
-    {
-      if 1 <= Capacity() {
-        data := data + [a];
+      if HasRemainingCapacity(1) {
+        data := data + [n];
         return Success(1);
       } else {
-        return Failure("IO Error: Reached end of stream.");
+        return Failure("IO Error: Stream capacity exceeded.");
+      }
+    }
+
+    method WriteUInt16(n: uint16) returns (res: Result<nat>)
+      requires Valid()
+      modifies `data
+      ensures Valid()
+      ensures match res
+        case Success(lengthWritten) =>
+          && old(HasRemainingCapacity(2))
+          && lengthWritten == 2
+          && data == old(data) + UInt16ToSeq(n)
+        case Failure(e) => unchanged(`data)
+    {
+      if HasRemainingCapacity(2) {
+        data := data + UInt16ToSeq(n);
+        return Success(2);
+      } else {
+        return Failure("IO Error: Stream capacity exceeded.");
+      }
+    }
+
+    method WriteUInt32(n: uint32) returns (res: Result<nat>)
+      requires Valid()
+      modifies `data
+      ensures Valid()
+      ensures match res
+        case Success(lengthWritten) =>
+          && old(HasRemainingCapacity(4))
+          && lengthWritten == 4
+          && data == old(data) + UInt32ToSeq(n)
+        case Failure(e) => unchanged(`data)
+    {
+      if HasRemainingCapacity(4) {
+        data := data + UInt32ToSeq(n);
+        return Success(4);
+      } else {
+        return Failure("IO Error: Stream capacity exceeded.");
       }
     }
   }
